examples/miniML/semantics/MiniMLTerminationScript.sml
@@ -104,7 +104,7 @@ val _ = register "type_subst" type_subst_def type_subst_ind;
 
 val (deBruijn_subst_def, deBruijn_subst_ind) =
   tprove_no_defn ((deBruijn_subst_def, deBruijn_subst_ind),
-  WF_REL_TAC `measure (λ(x,y). t_size y)` >>
+  WF_REL_TAC `measure (λ(_,x,y). t_size y)` >>
   rw [] >|
   [induct_on `ts'` >>
        rw [t_size_def] >>
